\documentclass{article}
\usepackage[utf8]{inputenc}
\usepackage{amsmath}

\author{Krystal Maughan }
\date{May 4th 2017}

\begin{document}

\section{Disjunctive Conjunction}
$\mathbf{Homework 3.3.2.1}$
\\
\\
Pick the predicate that best describes the operation:
\\
1.$ (x \leq 0 \land c = \hat{c} + 1) \vee (x > 0 \land c = \hat{c})$
\\
2.$ (x \leq y \land z = y) \vee (x \geq y \land z = x)$
\\
3.$ (x \leq y \land z = x) \vee (x \geq y \land z = y)$
\\
4.$ (x \geq 0 \land z = x) \vee (x \leq 0 \land z = -x)$
\\
5.$ (x \geq y \land z = x - y) \vee (y \geq x \land z = y - x)$
\\
\\
3.3.2.1-1: $z = abs(x)$
\\
$(x \geq 0 \land z = x) \vee (x \leq 0 \land z = -x)$
\\
\\
3.3.2.1-2: $z = min(x, y)$
\\
$(x \leq y \land z = x) \vee (x \geq y \land z = y)$
\\
\\
3.3.2.1-3: $z = max(x, y)$
\\
$(x \leq y \land z = y) \vee (x \geq y \land z = x)$
\\
\\
3.3.2.1-4: $z = abs(x - y)$
\\
$(x \geq y \land z = x - y) \vee (y \geq x \land z = y - x)$
\\
\\
3.3.2.1-5: Increment $c$ by one if $ x \leq 0$
\\
$(x \leq 0 \land c = \hat{c} + 1) \vee (x > 0 \land c = \hat{c})$

\end{document}
